coq/Sets.v
@@ -1,55 +1,15 @@
 Require Export Coq.Classes.EquivDec
         Coq.Lists.List Coq.Bool.Bool
-        Coq.Logic.FunctionalExtensionality.
+        Coq.Sorting.Permutation
+        CoqRecon.Base.
 Export ListNotations.
-
-Ltac inv H := inversion H; subst; clear H.
-
-Lemma contrapositive : forall P Q : Prop,
-    (P -> Q) -> ~ Q -> ~ P.
-Proof.
-  intuition.
-Qed.
-
-Lemma nexists_forall_not : forall {A : Type} (P : A -> Prop),
-    ~ (exists x, P x) -> forall x, ~ P x.
-Proof.
-  eauto.
-Qed.
-
-Section Curry.
-  Context {A B C : Type}.
-
-  Definition curry (f : A * B -> C) (a : A) (b : B) : C := f (a,b).
-
-  Definition uncurry (f : A -> B -> C) '((a,b) : A * B) : C := f a b.
-
-  Local Hint Unfold curry : core.
-  Local Hint Unfold uncurry : core.
-
-  Lemma curry_uncurry : forall f ab,
-      uncurry (curry f) ab = f ab.
-  Proof.
-      intros f [a b]; reflexivity.
-  Qed.
-
-  Lemma uncurry_curry : forall f a b,
-      curry (uncurry f) a b = f a b.
-  Proof.
-    reflexivity.
-  Qed.
-End Curry.
-
-Definition reflects
-           {A B : Type} (R : A -> B -> Prop) (f: A -> B -> bool) :=
-  forall a b, reflect (R a b) (f a b).
 
 Declare Scope set_scope.
 Delimit Scope set_scope with set.
 
-Reserved Notation "l ∪ r" (at level 50, left associativity).
-Reserved Notation "l ∩ r" (at level 49, left associativity).
-Reserved Notation "l ∖ r" (at level 48, left associativity).
+Reserved Notation "l ∪ r" (at level 45, left associativity).
+Reserved Notation "l ∩ r" (at level 44, left associativity).
+Reserved Notation "l ∖ r" (at level 43, left associativity).
 
 Section Sets.
   Context {A : Set}.
@@ -59,6 +19,20 @@ Section Sets.
     forall a, In a l -> In a r.
 
   Local Hint Unfold Subset : core.
+
+  Lemma Subset_perm_l : forall l l',
+      Permutation l' l ->
+      forall r, Subset l r -> Subset l' r.
+  Proof.
+    eauto using Permutation_in.
+  Qed.
+
+  Lemma Subset_perm_r : forall r r',
+      Permutation r r' ->
+      forall l, Subset l r -> Subset l r'.
+  Proof.
+    eauto using Permutation_in.
+  Qed.
   
   (** [u] is the union of [l] & [r]. *)
   Definition Union (l r u : list A) : Prop :=
@@ -154,7 +128,7 @@ Section Sets.
     rewrite H in Hmem. discriminate.
   Qed.
 
-  Lemma Not_In_member_ff : forall a l,
+  Lemma Not_In_member_iff : forall a l,
       ~ In a l <-> member a l = false.
   Proof.
     intros a l.
@@ -250,125 +224,43 @@ End Sets.
 
 Notation "l ⊆ r"
   := (Subset l r)
-       (at level 50, no associativity) : set_scope.
+       (at level 80, no associativity) : set_scope.
 Notation "l ∪ r" := (l ++ r) : set_scope.
 Notation "l ∩ r" := (intersect l r) : set_scope.
 Notation "l ∖ r" := (difference l r) : set_scope.
 
-Section Env.
-  Context {K V : Set}.
+Section SubsetUnion.
+  Open Scope set_scope.
 
-  Definition env : Set := K -> option V.
+  Context {A : Set}.
 
-  Definition empty : env := fun _ => None.
-  
-  Context {HDK : EqDec K eq}.
+  Hint Rewrite in_app_iff : core.
+  Local Hint Unfold Subset : core.
 
-  Definition bind (k : K) (v : V) (e : env) : env :=
-    fun k' => if equiv_dec k' k then Some v else e k'.
-
-  Lemma bind_sound : forall k v e,
-      (bind k v e) k = Some v.
+  Lemma Subset_cons : forall l r : list A,
+      l ⊆ r -> forall a : A, a :: l ⊆ a :: r.
   Proof.
-    intros k v e; unfold bind.
-    destruct (equiv_dec k k) as [Hk | Hk];
-      unfold equiv in *; try contradiction.
-    reflexivity.
-  Qed.
-
-  Lemma bind_complete : forall k' k v e,
-      k' <> k -> (bind k v e) k' = e k'.
-  Proof.
-    intros k' k v e Hk'k; unfold bind.
-    destruct (equiv_dec k' k) as [Hk | Hk];
-      unfold equiv in *; try contradiction.
-    reflexivity.
-  Qed.
-
-  Definition find (k : K) (e : env) : option V := e k.
-
-  Definition bound (k : K) (v : V) (e : env) : Prop := e k = Some v.
-
-  Definition mask (e : env) (ks : list K) : env :=
-    fun k => if member k ks then None else e k.
-
-  Definition dom (e : env) (d : list K) : Prop :=
-    forall k, In k d <-> exists v, e k = Some v.
-
-  Lemma env_binds : forall (k : K) (e : env),
-      e k = None \/ exists v, e k = Some v.
-  Proof.
-    intros k e.
-    destruct (e k) eqn:Heq; eauto.
+    unfold Subset; intros;
+      simpl in *; intuition.
   Qed.
   
-  Lemma dom_nil : forall e, dom e [] -> e = empty.
+  Lemma Subset_union_distr_l : forall l r : list A,
+      l ⊆ r -> forall s, s ∪ l ⊆ s ∪ r.
   Proof.
-    unfold dom. intros e H.
-    extensionality k. unfold empty.
-    specialize H with k.
-    destruct (env_binds k e) as [He | He]; auto.
-    apply H in He. inv He.
+    unfold Subset; intros.
+    autorewrite with core in *; intuition.
   Qed.
 
-  Lemma not_in_dom : forall k d e,
-      dom e d -> ~ In k d -> e k = None.
+  Lemma Subset_union_distr_r : forall l r : list A,
+      l ⊆ r -> forall s, l ∪ s ⊆ r ∪ s.
   Proof.
-    intros k d e Hdom HIn; unfold dom in *.
-    specialize Hdom with k.
-    destruct Hdom as [_ Hd].
-    pose proof contrapositive _ _ Hd as H.
-    apply H in HIn.
-    pose proof nexists_forall_not _ HIn as HE.
-    destruct (env_binds k e) as [Hk | [v Hk]]; auto.
-    apply HE in Hk. contradiction.
+    unfold Subset; intros.
+    autorewrite with core in *; intuition.
   Qed.
-
-  Definition range (e : env) (r : list V) : Prop :=
-    forall v, In v r <-> exists k, e k = Some v.
-End Env.
-
-Section EnvMap.
-  Context {A B C : Set}.
-  Variable (f : B -> C).
-  Context {HDK : EqDec A eq}.
-
-  Definition env_map (e : @env A B) : @env A C :=
-    fun a => match e a with
-          | Some b => Some (f b)
-          | None => None
-          end.
-
-  Lemma env_map_bind : forall a b e,
-      bind a (f b) (env_map e) = env_map (bind a b e).
+  
+  Lemma union_perm : forall l r : list A,
+      Permutation (l ∪ r) (r ∪ l).
   Proof.
-    intros a b e; extensionality k.
-    unfold bind, env_map.
-    destruct (equiv_dec k a) as [Hka | Hka];
-      unfold equiv in *; subst; reflexivity.
+    auto using Permutation_app_comm.
   Qed.
-End EnvMap.
-
-Section ComposeEnv.
-  Context {A B C : Set}.
-
-  Definition env_compose (eb : @env B C) (ea : @env A B) : @env A C :=
-    fun a => match ea a with
-          | Some b => eb b
-          | None => None
-          end.
-End ComposeEnv.
-
-Declare Scope env_scope.
-Delimit Scope env_scope with env.
-
-Notation "'∅'" := empty (at level 0, no associativity) : env_scope.
-Notation "k ↦ v ';;' e"
-  := (bind k v e)
-       (at level 11, right associativity) : env_scope.
-Notation "e ∉ ks"
-  := (mask e ks)
-       (at level 15, left associativity) : env_scope.
-Notation "eb ≺ ea"
-  := (env_compose eb ea)
-       (at level 14, left associativity) : env_scope.
+End SubsetUnion.
