coq/Base.v
@@ -1,0 +1,42 @@
+Require Export Coq.Bool.Bool.
+
+Ltac inv H := inversion H; subst; clear H.
+
+Lemma contrapositive : forall P Q : Prop,
+    (P -> Q) -> ~ Q -> ~ P.
+Proof.
+  intuition.
+Qed.
+
+Lemma nexists_forall_not : forall {A : Type} (P : A -> Prop),
+    ~ (exists x, P x) -> forall x, ~ P x.
+Proof.
+  eauto.
+Qed.
+
+Section Curry.
+  Context {A B C : Type}.
+
+  Definition curry (f : A * B -> C) (a : A) (b : B) : C := f (a,b).
+
+  Definition uncurry (f : A -> B -> C) '((a,b) : A * B) : C := f a b.
+
+  Local Hint Unfold curry : core.
+  Local Hint Unfold uncurry : core.
+
+  Lemma curry_uncurry : forall f ab,
+      uncurry (curry f) ab = f ab.
+  Proof.
+      intros f [a b]; reflexivity.
+  Qed.
+
+  Lemma uncurry_curry : forall f a b,
+      curry (uncurry f) a b = f a b.
+  Proof.
+    reflexivity.
+  Qed.
+End Curry.
+
+Definition reflects
+           {A B : Type} (R : A -> B -> Prop) (f: A -> B -> bool) :=
+  forall a b, reflect (R a b) (f a b).
