coq/Maybe.v
@@ -1,0 +1,33 @@
+Require Export Coq.Program.Utils Coq.Program.Basics.
+
+Section Maybe.
+  Context {A B : Type}.
+
+  Definition obind (f : A -> option B) (o : option A) : option B :=
+    match o with
+    | Some a => f a
+    | None => None
+    end.
+
+  Definition omap (f : A -> B) : option A -> option B :=
+    obind (Some ∘ f)%prg.
+End Maybe.
+
+Declare Scope maybe_scope.
+Delimit Scope maybe_scope with maybe.
+
+Notation "o '>>=' f"
+  := (obind f o)
+       (at level 50, left associativity) : maybe_scope.
+Notation "o '>>|' f"
+  := (omap f o)
+       (at level 50, left associativity) : maybe_scope.
+Notation "a '<-' o ';;' b"
+  := (obind (fun a => b) o)
+       (at level 60, right associativity) : maybe_scope.
+Notation "a '↤' o ';;' b"
+  := (omap (fun a => b) o)
+       (at level 60, right associativity) : maybe_scope.
+
+Ltac maybe_simpl :=
+  unfold ">>|","∘",">>=",omap,obind; simpl.
