coq/MonoCompleteness.v
@@ -1,0 +1,154 @@
+Require Export CoqRecon.Mono.
+
+(** Completeness is never true :(. *)
+
+Section Complete.
+  Local Hint Resolve sound : core.
+  Local Hint Resolve preservation : core.
+  Local Hint Resolve Subset_perm_l : core.
+  Local Hint Resolve Subset_perm_r : core.
+  Local Hint Resolve union_perm : core.
+  Local Hint Constructors Permutation : core.
+
+  Lemma tvars_subset : forall Γ e τ X C,
+      Γ ⊢ e ∈ τ ⊣ X @ C -> (Ctvars C ⊆ X)%set.
+  Proof.
+    intros g e t X C H; induction H;
+      simpl; try firstorder.
+    - apply Subset_perm_l
+        with (T :: tvars τ1 ∪ tvars τ2 ∪ Ctvars (C1 ∪ C2))%set.
+      + rewrite <- app_assoc with (m := [T]); simpl.
+        apply Permutation_sym. rewrite app_assoc.
+        apply Permutation_middle.
+      + apply Subset_cons. (** Dang. *) admit.
+    - (** Same problem. *) admit.
+    - (** Same problem. *) admit.
+  Abort.
+
+  (* Pierce's proof in TAPL relies upon this assumption. *)
+  Lemma tsub_inverse : forall t s,
+      exists t', (s † t')%typ = t /\ forall n, In n (tvars t') -> s n = None.
+  Proof.
+    intros t s;
+      induction t as
+        [| | t1 [t1' [IHt1 IHs1]] t2 [t2' [IHt2 IHs2]] | m].
+    - exists TBool; intuition.
+    - exists TNat; intuition.
+    - exists (t1' → t2')%typ; simpl.
+      rewrite IHt1, IHt2.
+      split; [reflexivity |].
+      intros n H. rewrite in_app_iff in H.
+      intuition.
+    - destruct (env_binds m s) as [HNone | [t HSome]].
+      + exists (TVar m); simpl. rewrite HNone.
+        intuition; subst; assumption.
+      + (* Which is difficult to formally verify...*)
+  Abort.
+
+  (** I used Pierce's [CT-Abs-Inf] rule
+      in place of [CT-Abs].
+      It seems his form of completenss is impossible
+      with this... *)
+  Theorem complete_weak : forall Γ e t X C,
+    Γ ⊢ e ∈ t ⊣ X @ C ->
+    forall σ τ,
+      (σ × Γ)%env ⊨ e ∈ τ ->
+      (forall m, In m X -> σ m = None) ->
+      exists σ', Forall (uncurry (satisfy σ')) C /\
+            (σ' † t = τ)%typ /\ (σ' ∉ X = σ)%env.
+  Proof.
+    intros g e τ X C H; induction H;
+      intros s t Ht Hd; inv Ht;
+        try (exists s; intuition; assumption).
+    - exists s; intuition.
+      unfold bound,env_map in *.
+      rewrite H in H1. inv H1.
+      reflexivity.
+    - (* This case is intractable.
+         There is no way to use the induction hypothesis. *)
+      admit.
+    - apply IHconstraint_typing1 in H7 as IH1;
+        [clear IHconstraint_typing1 H7 | intuition].
+      apply IHconstraint_typing2 in H9 as IH2;
+        [clear IHconstraint_typing2 H9 | intuition].
+      destruct IH1 as [s1 [HC1 [Ht1 Hs1]]].
+      destruct IH2 as [s2 [HC2 [Ht2 Hs2]]].
+      assert (HX12: member T X1 = false /\ member T X2 = false).
+      { repeat rewrite <- Not_In_member_iff; split;
+          intros ?; apply H2; repeat rewrite in_app_iff;
+            intuition. }
+      destruct HX12 as [HX1 HX2].
+      exists (fun Y =>
+           if Y == T then Some t else
+             if member Y X1 then s1 Y else
+               if member Y X2 then s2 Y else s Y).
+      repeat split.
+      + constructor; simpl.
+        * unfold satisfy; simpl.
+          destruct (equiv_dec T T) as [HTT | HTT];
+            unfold equiv, complement in *; try contradiction; simpl.
+          (* Need induction...probably...*) admit.
+        * rewrite Forall_app; split.
+          -- (* Need induction. *) admit.
+          -- (* Need induction. *) admit.
+      + simpl; destruct (equiv_dec T T) as [HTT | HTT];
+          unfold equiv, complement in *;
+          try contradiction; simpl; reflexivity.
+      + extensionality Y; unfold "∉"; simpl.
+        destruct (equiv_dec Y T) as [HYT | HYT];
+          unfold equiv, complement in *; subst.
+        * symmetry; apply Hd; intuition.
+        * destruct (member Y (X1 ∪ X2))%set eqn:HYmem;
+            simpl; auto.
+          -- symmetry; apply Hd. 
+             right; auto using member_In.
+          -- assert (HY1: member Y X1 = false).
+             rewrite <- Not_In_member_iff in *.
+             intuition. rewrite HY1.
+             assert (HY2: member Y X2 = false).
+             rewrite <- Not_In_member_iff in *.
+             intuition. rewrite HY2.
+             reflexivity.
+    - apply IHconstraint_typing1 in H8 as IH1;
+        [ clear IHconstraint_typing1 H8 | intuition ].
+      apply IHconstraint_typing2 in H10 as IH2;
+        [ clear IHconstraint_typing2 H10 | intuition ].
+      apply IHconstraint_typing3 in H11 as IH3;
+        [ clear IHconstraint_typing3 H11 | intuition ].
+      destruct IH1 as [s1 [HC1 [Ht1 Hs1]]].
+      destruct IH2 as [s2 [HC2 [Ht2 Hs2]]].
+      destruct IH3 as [s3 [HC3 [Ht3 Hs3]]].
+      exists (fun Y =>
+           if member Y X1 then s1 Y else
+             if member Y X2 then s2 Y else
+               if member Y X3 then s3 Y else s Y).
+      repeat split.
+      + repeat constructor.
+        * unfold satisfy, uncurry; simpl.
+          (* Requires induction... *) admit.
+        * unfold satisfy, uncurry; simpl.
+          (* Requires induction... *) admit.
+        * repeat rewrite Forall_app; repeat split.
+          (* Requires induction...*) admit. admit. admit.
+      + (* Nope. *) admit.
+      + extensionality Y; unfold "∉"; simpl.
+        destruct (member Y (X1 ∪ X2 ∪ X3)%set) eqn:HYmem.
+        * symmetry; apply Hd; auto using member_In.
+        * assert (HY123:
+                    member Y X1 = false /\
+                    member Y X2 = false /\
+                    member Y X3 = false).
+          { repeat rewrite <- Not_In_member_iff in *.
+            repeat rewrite in_app_iff in HYmem.
+            intuition. }
+          destruct HY123 as [HY1 [HY2 HY3]].
+          rewrite HY1,HY2,HY3. reflexivity.
+      + apply Hd;
+          repeat rewrite in_app_iff;
+          intuition.
+      + apply Hd;
+          repeat rewrite in_app_iff;
+          intuition.
+    - (* Same stuff... *)
+  Abort.
+End Complete.
